Huge overhaul. Checkpoint.

theories/FreeVariables.v
@@ -2,18 +2,10 @@ From Coq Require Export
   Lists.List.
 Export ListNotations.
 From Lang Require Import
+  StructuralFreeVariables
   Invert
   Partition
   Terms.
-
-Fixpoint remove_all x li :=
-  match li with
-  | [] => []
-  | hd :: tl =>
-      let recursed := remove_all x tl in
-      if eqb x hd then recursed else hd :: recursed
-  end.
-(* tail-recursive version flips the order *)
 
 Definition remove_if_head x li :=
   match li with
@@ -22,7 +14,7 @@ Definition remove_if_head x li :=
   end.
 Arguments remove_if_head x/ li.
 
-Fixpoint fv_with rm t :=
+Fixpoint fv t :=
   match t with
   | TmVoid
   | TmStar _
@@ -31,19 +23,17 @@ Fixpoint fv_with rm t :=
   | TmVarS s =>
       [s]
   | TmAppl f x =>
-      fv_with rm f ++ fv_with rm x
+      fv f ++ fv x
   | TmPack _ arg ty curry
   | TmForA arg ty curry =>
       let lo := (
-        let recursed := fv_with rm curry in
+        let recursed := fv curry in
         match arg with
         | None => recursed
-        | Some a => rm a recursed
+        | Some a => remove_if_head a recursed
         end) in
-      partition_pf eqb (fv_with remove_all (* <-- yes, hard-code this *) ty) lo ++ lo
+      partition_pf eqb (structural_fv ty) lo ++ lo
   end.
-Definition fv := fv_with remove_if_head.
-Arguments fv/ t.
 
 (* Crucial distinction from an easier-to-implement algorithm! *)
 Example fv_permits_shadowing : forall x,
@@ -109,56 +99,6 @@ Qed.
 Definition fv := fv_fast [].
 *)
 
-Inductive Wherever {T} (x : T) : list T -> list T -> Prop :=
-  | WhereverNil :
-      Wherever x [] []
-  | WhereverHere : forall a b,
-      Wherever x a b ->
-      Wherever x a (x :: b)
-  | WhereverSkip : forall hd tla tlb,
-      x <> hd ->
-      Wherever x tla tlb ->
-      Wherever x (hd :: tla) (hd :: tlb)
-  .
-
-Example wherever_12345 : Wherever 9 [1;2;3;4;5] [9;1;9;9;2;3;9;4;9;9;9;9;5;9].
-Proof. repeat constructor; intro C; discriminate C. Qed.
-
-Lemma wherever_refl : forall {T} (x : T) li,
-  (~In x li) ->
-  Wherever x li li.
-Proof.
-  induction li; constructor; apply Decidable.not_or in H as [H I]. { symmetry. assumption. } apply IHli. assumption.
-Qed.
-
-Lemma wherever_not_in_orig : forall {T} (x : T) li post,
-  Wherever x li post ->
-  ~In x li.
-Proof.
-  intros T x li post H C. generalize dependent C. generalize dependent post. generalize dependent x.
-  induction li; intros; destruct C; subst.
-  - remember (x :: li) as xli eqn:Ex. induction H; intros.
-    { discriminate. } { apply IHWherever. assumption. } invert Ex. apply H. reflexivity.
-  - remember (a :: li) as ali eqn:Ea. generalize dependent a. generalize dependent li. induction H; intros.
-    { discriminate. } { eapply IHWherever. { apply IHli. } { assumption. } apply Ea. }
-    invert Ea. eapply IHli. { apply H0. } assumption.
-Qed.
-
-Lemma wherever_remove_all : forall x li post,
-  Wherever x li post <-> remove_all x post = li.
-Proof.
-  split; intros.
-  - induction H.
-    + reflexivity.
-    + simpl. rewrite eqb_refl. assumption.
-    + simpl. apply eqb_neq in H. rewrite H. f_equal. assumption.
-  - generalize dependent x. generalize dependent li. induction post; intros.
-    + invert H. constructor.
-    + simpl in H. destruct (eqb x a) eqn:E.
-      * apply eqb_eq in E. subst. constructor. apply IHpost. reflexivity.
-      * apply eqb_neq in E. subst. constructor. { assumption. } apply IHpost. reflexivity.
-Qed.
-
 Variant MaybeCons {T} (hd : T) : list T -> list T -> Prop :=
   | MaybeConsNil :
       MaybeCons hd [] []
@@ -182,81 +122,47 @@ Proof.
     + destruct (eqb_spec x s); subst; constructor. assumption.
 Qed.
 
-Inductive FreeInWith : (string -> list string -> list string -> Prop) -> term -> list string -> Prop :=
-  | FreeVoid : forall cmp,
-      FreeInWith cmp TmVoid []
-  | FreeStar : forall cmp univ,
-      FreeInWith cmp (TmStar univ) []
-  | FreeAtom : forall cmp id,
-      FreeInWith cmp (TmAtom id) []
-  | FreeVarS : forall cmp x,
-      FreeInWith cmp (TmVarS x) [x]
-  | FreePack : forall cmp id arg ty curry va vb avb v pf,
-      FreeInWith Wherever ty va ->
-      FreeInWith cmp curry avb ->
+Inductive FreeIn : term -> list string -> Prop :=
+  | FreeVoid :
+      FreeIn TmVoid []
+  | FreeStar : forall univ,
+      FreeIn (TmStar univ) []
+  | FreeAtom : forall id,
+      FreeIn (TmAtom id) []
+  | FreeVarS : forall x,
+      FreeIn (TmVarS x) [x]
+  | FreePack : forall id arg ty curry v,
+      FreeIn (TmForA    arg ty curry) v ->
+      FreeIn (TmPack id arg ty curry) v
+  | FreeForA : forall arg ty curry va vb avb v pf,
+      StructurallyFreeIn ty va ->
+      FreeIn curry avb ->
       Partition pf va vb ->
       v = pf ++ vb ->
-      (match arg with None => eq | Some a => cmp a end) vb avb ->
-      FreeInWith cmp (TmPack id arg ty curry) v
-  | FreeForA : forall cmp arg ty curry va vb avb v pf,
-      FreeInWith Wherever ty va ->
-      FreeInWith cmp curry avb ->
-      Partition pf va vb ->
-      v = pf ++ vb ->
-      (match arg with None => eq | Some a => cmp a end) vb avb ->
-      FreeInWith cmp (TmForA arg ty curry) v
-  | FreeAppl : forall cmp f x va vb v,
-      FreeInWith cmp f va ->
-      FreeInWith cmp x vb ->
+      (match arg with None => eq | Some a => MaybeCons a end) vb avb ->
+      FreeIn (TmForA arg ty curry) v
+  | FreeAppl : forall f x va vb v,
+      FreeIn f va ->
+      FreeIn x vb ->
       va ++ vb = v ->
-      FreeInWith cmp (TmAppl f x) v
+      FreeIn (TmAppl f x) v
   .
-Definition FreeIn := FreeInWith MaybeCons.
-Arguments FreeIn/ t vs.
+Arguments FreeIn t vs.
 
 Definition Closed := fun t => FreeIn t [].
 Arguments Closed t/.
-
-Lemma map_distr : forall {A B} (f : A -> B) hd tl, map f (hd ++ tl) = map f hd ++ map f tl.
-Proof.
-  intros. generalize dependent tl. generalize dependent B.
-  induction hd; intros; simpl in *; try rewrite IHhd; reflexivity.
-Qed.
 
 Theorem slow_down : forall {T} f hi lo,
   rev' (@partition_pf_fast T [] f hi lo) = partition_pf_slow f hi lo.
 Proof. intros. rewrite <- partition_pf_fast_slow. reflexivity. Qed.
 
-Theorem reflect_fv_structural : forall t v,
-  fv_with remove_all t = v <-> FreeInWith Wherever t v.
+Theorem reflect_fv : forall t v,
+  (fv t = v <-> FreeIn t v).
 Proof.
   split; intros.
-  - generalize dependent v. induction t; intros; subst; simpl in *; repeat rewrite slow_down; try solve [constructor];
-    [| | econstructor; [apply IHt1 | apply IHt2 |]; reflexivity];
-    destruct arg; (econstructor; [apply IHt1 | apply IHt2 | | |]);
-    try reflexivity; try apply wherever_remove_all; try reflexivity;
-    rewrite <- partition_pf_fast_slow; apply partition_pf_works; apply eqb_spec.
-  - remember Wherever as cmp eqn:Ec. generalize dependent Ec.
-    induction H; intros; subst; simpl in *; try reflexivity; repeat rewrite slow_down;
-    specialize (IHFreeInWith1 eq_refl); specialize (IHFreeInWith2 eq_refl); subst; [| | reflexivity];
-    destruct arg; repeat rewrite wherever_remove_all in *; subst; f_equal;
-    rewrite <- partition_pf_fast_slow; apply (reflect_partition_pf _ _ _ _ eqb_spec); assumption.
-Qed.
-
-Theorem reflect_fv : forall Cmp cmp t v,
-  (forall a b z, Cmp a z b <-> cmp a b = z) ->
-  (fv_with cmp t = v <-> FreeInWith Cmp t v).
-Proof.
-  split; intros.
-  - generalize dependent Cmp. generalize dependent cmp. generalize dependent v.
-    induction t; intros; subst; simpl in *; repeat rewrite slow_down; try solve [constructor];
-    [| | econstructor; [apply (IHt1 _ _ eq_refl _ H) | apply (IHt2 _ _ eq_refl _ H) | reflexivity]];
-    destruct arg; (econstructor; [apply reflect_fv_structural; reflexivity | apply (IHt2 _ _ eq_refl _ H) | | reflexivity |]);
-    try apply H; try reflexivity; rewrite <- partition_pf_fast_slow; apply partition_pf_works; apply eqb_spec.
-  - generalize dependent cmp.
-    induction H0; intros; subst; simpl in *; try reflexivity; repeat rewrite slow_down;
-    [| | rewrite (IHFreeInWith1 _ H0); rewrite (IHFreeInWith2 _ H0); reflexivity];
-    (destruct arg; [apply H2 in H1 |]); subst; simpl in *; (rewrite IHFreeInWith2; [f_equal | assumption]);
-    rewrite <- partition_pf_fast_slow; apply (reflect_partition_pf _ _ _ _ eqb_spec);
-    (rewrite IHFreeInWith1; [assumption |]); intros; apply wherever_remove_all.
+  - generalize dependent v. induction t; intros; subst; simpl in *; try solve [constructor]; [constructor | |];
+    econstructor; try apply reflect_structural_fv; try apply IHt1; try apply IHt2; try reflexivity;
+    try apply (partition_pf_works _ _ _ eqb_spec); (destruct arg; [apply maybe_cons_remove_if_head |]); reflexivity.
+  - induction H; subst; simpl in *; try reflexivity. eapply (reflect_partition_pf _ _ _ _ eqb_spec) in H1.
+    apply reflect_structural_fv in H. destruct arg; [apply maybe_cons_remove_if_head in H3 |]; subst; reflexivity.
 Qed.
