theories/Subst.v
@@ -1,46 +1,14 @@
-From Coq Require Import
-  Lists.List.
-Import ListNotations.
+From Coq Require Export
+  List.
+Export ListNotations.
 From Lang Require Import
   FreeVariables
+  FstCmp
   Invert
   Partition
+  StructuralFreeVariables
+  StructuralSubst
   Terms.
-
-Fixpoint smap
-  (f : (term -> term) -> term -> term)
-  (x : list (string * (term -> term))) :
-  list (string * (term -> term)) :=
-  match x with
-  | [] => []
-  | (s, g) :: tl => (s, f g) :: smap f tl
-  end.
-
-Theorem smap_distr : forall f a b,
-  smap f (a ++ b) = smap f a ++ smap f b.
-Proof.
-  intros f a. generalize dependent f. induction a; intros; simpl in *.
-  { reflexivity. } destruct a. rewrite IHa. reflexivity.
-Qed.
-
-Theorem smap_len : forall f li,
-  Datatypes.length (smap f li) = Datatypes.length li.
-Proof.
-  intros f li. generalize dependent f. induction li; intros; simpl in *.
-  { reflexivity. } destruct a. simpl. rewrite IHli. reflexivity.
-Qed.
-
-Theorem map_fst_smap : forall f li,
-  map fst (smap f li) = map fst li.
-Proof. induction li. { reflexivity. } destruct a. simpl. rewrite IHli. reflexivity. Qed.
-
-Fixpoint remove_key_all {T} x (li : list (string * T)) :=
-  match li with
-  | [] => []
-  | (s, f) :: tl =>
-      let recursed := remove_key_all x tl in
-      if eqb x s then recursed else (s, f) :: recursed
-  end.
 
 Definition remove_key_if_head {T} x (li : list (string * T)) :=
   match li with
@@ -48,27 +16,11 @@ Definition remove_key_if_head {T} x (li : list (string * T)) :=
   | (s, f) :: tl => if eqb x s then tl else li
   end.
 
-Lemma remove_all_key_eq : forall {T} x (li : list (string * T)),
-  map fst (remove_key_all x li) = remove_all x (map fst li).
-Proof.
-  intros. generalize dependent x. induction li; intros; simpl in *. { reflexivity. }
-  destruct a. simpl. destruct (eqb x s) eqn:E. { apply IHli. } simpl. f_equal. apply IHli.
-Qed.
-
 Lemma remove_if_head_key_eq : forall {T} x (li : list (string * T)),
   map fst (remove_key_if_head x li) = remove_if_head x (map fst li).
 Proof.
   intros. generalize dependent x. induction li; intros; simpl in *. { reflexivity. }
   destruct a. simpl. destruct (eqb x s) eqn:E. { reflexivity. } simpl. reflexivity.
-Qed.
-
-Lemma remove_key_all_eq : forall {T} x li,
-  ~In x (map fst li) ->
-  @remove_key_all T x li = li.
-Proof.
-  intros. generalize dependent x. induction li; intros; simpl in *. { reflexivity. }
-  destruct a. simpl in *. apply Decidable.not_or in H as [H1 H2]. apply eqb_neq in H1.
-  rewrite eqb_sym in H1. rewrite H1. f_equal. apply IHli. assumption.
 Qed.
 
 Theorem incl_remove_key : forall {T} x (li : list (string * T)),
@@ -85,7 +37,7 @@ Qed.
 
 (* Ludicrous that this is the easiest correct definition to write.
  * Generates substitution functions for every free variable at once. *)
-Fixpoint grand_unified_subst_with rm t : list (string * (term -> term)) :=
+Fixpoint grand_unified_subst t : list (string * (term -> term)) :=
   match t with
   | TmVoid
   | TmStar _
@@ -95,33 +47,25 @@ Fixpoint grand_unified_subst_with rm t : list (string * (term -> term)) :=
       [(s, fun x => x)]
   | TmPack id arg ty curry =>
       let lo := smap (fun f x => TmPack id arg ty (f x)) (
-        let recursed := grand_unified_subst_with rm curry in
+        let recursed := grand_unified_subst curry in
         match arg with
         | None => recursed
-        | Some a => rm a recursed
+        | Some a => remove_key_if_head a recursed
         end) in
-      let hi := smap (fun f x => TmPack id arg (f x) curry) (grand_unified_subst_with remove_key_all ty) in
+      let hi := smap (fun f x => TmPack id arg (f x) curry) (structural_grand_unified_subst ty) in
       partition_pf fst_cmp hi lo ++ lo
   | TmForA arg ty body =>
       let lo := smap (fun f x => TmForA arg ty (f x)) (
-        let recursed := grand_unified_subst_with rm body in
+        let recursed := grand_unified_subst body in
         match arg with
         | None => recursed
-        | Some a => rm a recursed
+        | Some a => remove_key_if_head a recursed
         end) in
-      let hi := smap (fun f x => TmForA arg (f x) body) (grand_unified_subst_with remove_key_all ty) in
+      let hi := smap (fun f x => TmForA arg (f x) body) (structural_grand_unified_subst ty) in
       partition_pf fst_cmp hi lo ++ lo
   | TmAppl a b =>
-      smap (fun f x => TmAppl (f x) b) (grand_unified_subst_with rm a) ++
-      smap (fun f x => TmAppl a (f x)) (grand_unified_subst_with rm b)
-  end.
-Definition grand_unified_subst := grand_unified_subst_with remove_key_if_head.
-Arguments grand_unified_subst/ t.
-
-Fixpoint pair_lookup {V} key (pairs : list (string * V)) :=
-  match pairs with
-  | [] => None
-  | (k, v) :: tl => if eqb key k then Some v else pair_lookup key tl
+      smap (fun f x => TmAppl (f x) b) (grand_unified_subst a) ++
+      smap (fun f x => TmAppl a (f x)) (grand_unified_subst b)
   end.
 
 Definition subst x y t := option_map (fun f => f y) (pair_lookup x (grand_unified_subst t)).
@@ -148,116 +92,21 @@ Lemma fst_cmp_eqb : forall {T} a a' b b',
   @fst_cmp T T (a, b) (a', b') = eqb a a'.
 Proof. reflexivity. Qed.
 
-Theorem grand_unified_subst_structural_fv : forall t,
-  fv_with remove_all t = map fst (grand_unified_subst_with remove_key_all t).
-Proof.
-  induction t; intros; subst; simpl in *; try reflexivity; repeat rewrite slow_down;
-  repeat rewrite IHt1; repeat rewrite IHt2; repeat rewrite map_distr; repeat rewrite map_fst_smap; [| | reflexivity];
-  destruct arg; f_equal; repeat rewrite <- partition_pf_fast_slow; try rewrite (map_fst_partition_pf _ _ _ _ fst_cmp_eqb);
-  repeat rewrite map_fst_smap; repeat rewrite remove_all_key_eq; reflexivity.
-Qed.
-
 Theorem grand_unified_subst_fv : forall t,
   fv t = map fst (grand_unified_subst t).
 Proof.
-  induction t; intros; simpl in *; try reflexivity; repeat rewrite slow_down;
-  repeat rewrite IHt1; repeat rewrite IHt2; repeat rewrite map_distr; repeat rewrite <- partition_pf_fast_slow;
-  repeat rewrite (map_fst_partition_pf _ _ _ _ fst_cmp_eqb); repeat rewrite map_fst_smap; [| | reflexivity];
-  repeat rewrite grand_unified_subst_structural_fv; (destruct arg; [| reflexivity]); repeat rewrite partition_pf_fast_slow;
-  (destruct (grand_unified_subst_with remove_key_if_head t2); [reflexivity |]);
-  destruct p as [v f]; simpl in *; destruct (eqb s v); reflexivity.
+  induction t; intros; simpl in *; try reflexivity; repeat rewrite slow_down; repeat rewrite <- partition_pf_fast_slow;
+  rewrite map_distr; try rewrite (map_fst_partition_pf _ _ _ _ fst_cmp_eqb); repeat rewrite map_fst_smap;
+  repeat rewrite IHt1; repeat rewrite IHt2; [| | reflexivity]; rewrite structural_grand_unified_subst_fv;
+  (destruct arg; [| reflexivity]); repeat rewrite partition_pf_fast_slow; (destruct (grand_unified_subst t2); [reflexivity |]);
+  destruct p as [v f]; simpl; destruct (eqb s v); reflexivity.
 Qed.
 (* WOOHOOOOOOOOOOOOOOO *)
-
-Lemma pair_lookup_smap : forall f x li,
-  pair_lookup x (smap f li) = option_map f (pair_lookup x li).
-Proof.
-  intros f x li. generalize dependent x. generalize dependent f.
-  induction li; intros; simpl in *. { reflexivity. }
-  destruct a. simpl. destruct (eqb x s) eqn:E. { reflexivity. } apply IHli.
-Qed.
-
-Lemma pair_lookup_app : forall {T} x a b,
-  @pair_lookup T x (a ++ b) =
-  match pair_lookup x a with
-  | None => pair_lookup x b
-  | Some out => Some out
-  end.
-Proof.
-  intros T x a. generalize dependent x. induction a; intros; simpl in *. { reflexivity. }
-  destruct a. destruct (eqb x s). { reflexivity. } apply IHa.
-Qed.
-
-Lemma pair_lookup_Forall_snd : forall {T} P li x y,
-  Forall P (map snd li) ->
-  @pair_lookup T x li = Some y ->
-  P y.
-Proof.
-  intros T P li x y Hf Hl. generalize dependent y. generalize dependent x.
-  remember (map snd li) eqn:Emap. generalize dependent li.
-  induction Hf; intros; destruct li; invert Emap; try discriminate Hl.
-  destruct p. simpl in *. destruct (eqb x0 s) eqn:E. { invert Hl. assumption. }
-  eapply IHHf; [reflexivity |]. apply Hl.
-Qed.
-
-Lemma pair_lookup_Forall : forall {T} P li x t,
-  Forall P li ->
-  @pair_lookup T x li = Some t ->
-  P (x, t).
-Proof.
-  intros T P li x t Hf Hl. generalize dependent t. generalize dependent x.
-  induction Hf; intros; simpl in *. { discriminate Hl. } destruct x as [k v].
-  destruct (eqb x0 k) eqn:E; [apply eqb_eq in E; invert Hl | apply IHHf]; assumption.
-Qed.
-
-Theorem Forall_smap : forall f P li,
-  Forall (fun p : _ * _ => let (x, g) := p in P (x, f g)) li ->
-  Forall P (smap f li).
-Proof.
-  intros. remember (fun p : string * (term -> term) => let (x, g) := p in P (x, f g)) as F eqn:EF.
-  generalize dependent P. generalize dependent f. induction H; intros; [apply Forall_nil |].
-  destruct x as [s g]. subst. simpl in *. constructor; [assumption |]. apply IHForall. reflexivity.
-Qed.
-
-Lemma remove_key_all_incl : forall {T} x (li : list (string * T)),
-  incl (remove_key_all x li) li.
-Proof.
-  unfold incl. intros T x li. generalize dependent x. induction li; intros; simpl in *. { destruct H. }
-  destruct a. destruct (eqb x s) eqn:E. { apply eqb_eq in E. subst. right. eapply IHli. apply H. }
-  destruct a0. destruct H. { left. assumption. } right. eapply IHli. apply H.
-Qed.
 
 Lemma remove_key_if_head_incl : forall {T} x (li : list (string * T)),
   incl (remove_key_if_head x li) li.
 Proof.
   unfold incl. intros T x [] [a1 a2] H. { inversion H. } destruct p. simpl in H. destruct (eqb x s); [right |]; assumption.
-Qed.
-
-(* God this is the dumbest function of all time but it's only ever used in proofs *)
-Fixpoint slow_unique_key {T} (li : list (string * T)) :=
-  match li with
-  | [] => []
-  | (s, t) :: tl => (s, t) :: remove_key_all s (slow_unique_key tl)
-  end.
-
-Lemma has_remove_key_all : forall {T} (x y : string * T) (li : list (string * T)),
-  fst_cmp x y = false ->
-  existsb (fst_cmp x) (remove_key_all (fst y) li) = existsb (fst_cmp x) li.
-Proof.
-  intros. generalize dependent y. generalize dependent x. induction li; intros; simpl in *. { reflexivity. }
-  destruct a. destruct x. destruct y. unfold fst_cmp in *. simpl in *.
-  destruct (eqb s1 s) eqn:E1. { apply eqb_eq in E1. subst. rewrite H. apply (IHli (s0, t0) (s, t)). assumption. }
-  destruct (eqb s0 s) eqn:E0; simpl in *. { rewrite E0. reflexivity. } rewrite E0. apply (IHli (s0, t0) (s1, t1)). assumption.
-Qed.
-
-Lemma has_slow_unique : forall {T} x li,
-  existsb (@fst_cmp T T x) (slow_unique_key li) = existsb (fst_cmp x) li.
-Proof.
-  intros T [s t] li. generalize dependent t. generalize dependent s.
-  induction li; intros; simpl in *. { reflexivity. }
-  destruct a. destruct (eqb_spec s s0). { subst. unfold fst_cmp. simpl. rewrite eqb_refl. reflexivity. }
-  simpl. rewrite (has_remove_key_all (s, t) (s0, t0)). 2: { unfold fst_cmp. simpl. apply eqb_neq. assumption. }
-  unfold fst_cmp. simpl. apply eqb_neq in n. rewrite n. apply (IHli _ t).
 Qed.
 
 Theorem incl_partition_pf_fst : forall {T} hi lo,
@@ -270,18 +119,6 @@ Proof.
   left. assumption.
 Qed.
 
-Theorem grand_unified_subst_structural_id : forall t,
-  let P := fun p : _ * _ => let (x, f) := p in f (TmVarS x) = t in
-  Forall P (grand_unified_subst_with remove_key_all t).
-Proof.
-  induction t as [| | | | id arg a IHa b IHb | arg a IHa b IHb | a IHa b IHb]; simpl in *; repeat constructor; [| |
-    apply Forall_app; split; apply Forall_smap; (eapply Forall_impl; [| try apply IHa; apply IHb]);
-    intros; destruct a0; rewrite H; reflexivity]; repeat rewrite slow_down; destruct arg;
-  apply Forall_app; (split; [eapply incl_Forall; [apply incl_partition_pf_fst |] |]); apply Forall_smap;
-  try (eapply incl_Forall; [apply remove_key_all_incl |]); (eapply Forall_impl; [| try apply IHa; apply IHb]);
-  intros; destruct a0; rewrite H; reflexivity.
-Qed.
-
 Theorem grand_unified_subst_id : forall t,
   let P := fun p : _ * _ => let (x, f) := p in f (TmVarS x) = t in
   Forall P (grand_unified_subst t).
@@ -291,7 +128,7 @@ Proof.
     intros; destruct a0; rewrite H; reflexivity]; repeat rewrite slow_down; destruct arg;
   apply Forall_app; (split; [eapply incl_Forall; [apply incl_partition_pf_fst |] |]);
   apply Forall_smap; try (eapply incl_Forall; [apply remove_key_if_head_incl |]);
-  (eapply Forall_impl; [| try apply grand_unified_subst_structural_id; apply IHb]);
+  (eapply Forall_impl; [| try apply structural_grand_unified_subst_id; apply IHb]);
   intros; destruct a0; rewrite H; reflexivity.
 Qed.
 
