theories/Values.v
@@ -1,31 +1,76 @@
+From Coq Require Export
+  List.
+Export ListNotations.
+From Coq Require
+  Program.Wf.
 From Lang Require Import
-  Terms
-  Types.
+  Invert
+  Terms.
 
 Inductive Value : term -> Prop :=
+  | ValStar : forall univ,
+      Value (TmStar univ)
   | ValAtom : forall id,
       Value (TmAtom id)
-  | ValPack : forall id arg arg_ty curry x ty,
-      let pack := TmPack id arg arg_ty curry in
-      let appl := TmAppl pack x in
-      Value x ->
-      Value curry ->
+  | ValPack : forall id arg ty curry,
       AtomId id curry ->
-      Typed [] appl ty ->
-      Value appl
-  | ValForA : forall arg arg_ty body ty,
-      let fora := TmForA arg arg_ty body in
+      Value (TmForA    arg ty curry) ->
+      Value (TmPack id arg ty curry)
+  | ValForA : forall arg ty body,
+      let fora := TmForA arg ty body in
+      Value ty ->
       Value body -> (* Consider removing this *)
-      Typed [] fora ty ->
       Value fora
+  | ValApplPack : forall id arg ty curry x,
+      let pack := TmPack id arg ty curry in
+      let appl := TmAppl pack x in
+      Value pack ->
+      Value x ->
+      Value appl
   .
 
-Theorem values_always_typed : forall v,
-  Value v ->
-  exists ty, Typed [] v ty.
+Fixpoint is_value t :=
+  match t with
+  | TmVoid
+  | TmVarS _ =>
+      false
+  | TmStar _
+  | TmAtom _ =>
+      true
+  | TmPack id arg ty curry =>
+      match atom_id curry with
+      | None => false
+      | Some aid => andb (eqb id aid) (andb (is_value ty) (is_value curry))
+      end
+  | TmForA arg ty body =>
+      andb (is_value ty) (is_value body)
+  | TmAppl (TmPack id arg ty curry) x =>
+      match atom_id curry with
+      | None => false
+      | Some aid => andb (is_value x) (andb (eqb id aid) (andb (is_value ty) (is_value curry)))
+      end
+  | TmAppl _ _ =>
+      false
+  end.
+
+Theorem reflect_value : forall t,
+  Bool.reflect (Value t) (is_value t).
 Proof.
-  intros. induction H.
-  - exists (TmAtom id). constructor.
-  - exists ty. assumption.
-  - exists ty. assumption.
+  induction t; simpl in *; repeat constructor; try solve [intro C; inversion C].
+  - destruct (atom_id t2) eqn:A. 2: {
+      constructor. intro C. invert C. eapply reflect_not_atom_id in A. apply A in H1 as []. }
+    destruct (eqb_spec id s). 2: {
+      constructor. intro C. invert C. apply reflect_atom_id in H1. rewrite A in H1. invert H1. apply n. reflexivity. }
+    subst. simpl. destruct IHt1. 2: { constructor. intro C. invert C. invert H4. apply n in H2 as []. }
+    destruct IHt2. 2: { constructor. intro C. invert C. invert H4. apply n in H5 as []. }
+    constructor. constructor. { apply reflect_atom_id. assumption. } constructor; assumption.
+  - destruct IHt1. 2: { constructor. intro C. invert C. apply n in H1 as []. }
+    destruct IHt2. 2: { constructor. intro C. invert C. apply n in H3 as []. }
+    constructor. constructor; assumption.
+  - destruct t1; try (constructor; intro C; inversion C). rename t1_1 into ty. rename t1_2 into curry. simpl in *.
+    destruct (atom_id curry) eqn:A. 2: { invert IHt1. constructor. intro C. invert C. apply H in H2 as []. }
+    destruct (eqb id s). 2: {
+      invert IHt1. simpl. rewrite Bool.andb_false_r. constructor. intro C. invert C. apply H in H2 as []. }
+    destruct IHt2. 2: { constructor. intro C. invert C. apply n in H5 as []. }
+    invert IHt1; constructor. { constructor; assumption. } intro C. invert C. apply H0 in H3 as [].
 Qed.
