theories/FstCmp.v
@@ -1,0 +1,23 @@
+From Coq Require Import
+  List
+  String.
+
+Definition ap_fst {A B C} : (A -> C) -> ((A * B) -> C) := fun f x => let (a, b) := x in f a.
+
+Lemma existsb_map_fst : forall {A B} li f f' x y,
+  (forall (a a' : A) (b b' : B), f (a, b) (a', b') = f' a a') ->
+  existsb (f (x, y)) li = existsb (f' x) (map fst li).
+Proof.
+  induction li; intros; simpl in *. { reflexivity. }
+  destruct a. simpl. rewrite H. destruct (f' x a). { reflexivity. } apply IHli. assumption.
+Qed.
+
+Definition fst_cmp {A B} := fun (a : string * A) (b : string * B) => eqb (fst a) (fst b).
+
+Lemma has_cmp_fst : forall {T} li s t,
+  existsb (@fst_cmp T T (s, t)) li = existsb (eqb s) (map fst li).
+Proof.
+  intros T li. induction li; intros; simpl in *. { reflexivity. }
+  destruct a. unfold fst_cmp. simpl in *. destruct (eqb s s0). { reflexivity. }
+  apply (IHli _ t).
+Qed.
