theories/Hole.v
@@ -1,0 +1,48 @@
+From Lang Require Import
+  Terms.
+
+Inductive hole : Set :=
+  | HoleHere
+  | HolePackTy (id : string) (arg : option string) (curry : term)
+  | HolePackCurry (id : string) (arg : option string) (ty : term)
+  | HoleForATy (arg : option string) (body : term)
+  | HoleForABody (arg : option string) (ty : term)
+  | HoleApplF (x : term)
+  | HoleApplX (f : term)
+  .
+
+Definition fill : hole -> term -> term := fun h t =>
+  match h with
+  | HoleHere => t
+  | HolePackTy id arg curry => TmPack id arg t curry
+  | HolePackCurry id arg ty => TmPack id arg ty t
+  | HoleForATy arg body => TmForA arg t body
+  | HoleForABody arg ty => TmForA arg ty t
+  | HoleApplF x => TmAppl t x
+  | HoleApplX f => TmAppl f t
+  end.
+
+Inductive Fill : hole -> term -> term -> Prop :=
+  | FillHere : forall t,
+      Fill HoleHere t t
+  | FillPackTy : forall id arg ty curry,
+      Fill (HolePackTy id arg curry) ty (TmPack id arg ty curry)
+  | FillPackCurry : forall id arg ty curry,
+      Fill (HolePackCurry id arg ty) curry (TmPack id arg ty curry)
+  | FillForATy : forall arg ty body,
+      Fill (HoleForATy arg body) ty (TmForA arg ty body)
+  | FillForABody : forall arg ty body,
+      Fill (HoleForABody arg ty) body (TmForA arg ty body)
+  | FillApplF : forall f x,
+      Fill (HoleApplF x) f (TmAppl f x)
+  | FillApplX : forall f x,
+      Fill (HoleApplX f) x (TmAppl f x)
+  .
+
+Theorem reflect_fill : forall h t t',
+  fill h t = t' <-> Fill h t t'.
+Proof.
+  split; intros.
+  - destruct h; subst; constructor.
+  - destruct H; reflexivity.
+Qed.
