theories/Step.v
@@ -1,0 +1,60 @@
+From Lang Require Import
+  Invert
+  PartitionKV
+  Subst
+  Terms
+  Values.
+
+Inductive Step : list (string * term) -> term -> list (string * term) -> term -> Prop :=
+  | StepVarS : forall id val,
+      Step [(id, val)] (TmVarS id) [] val
+  | StepPack : forall ctx arg ty curry ctx' arg' ty' curry' id,
+      Step ctx (TmForA arg ty curry) ctx' (TmForA arg' ty' curry') ->
+      Step ctx (TmPack id arg ty curry) ctx' (TmPack id arg' ty' curry')
+  | StepForATy : forall ctx ty ctx' ty' arg curry,
+      Step ctx ty ctx' ty' ->
+      Step ctx (TmForA arg ty curry) ctx' (TmForA arg ty' curry)
+  | StepForACurry : forall ctx curry ctx' curry' arg ty,
+      Step ctx curry ctx' curry' ->
+      Step ctx (TmForA arg ty curry) ctx' (TmForA arg ty curry')
+  | StepForAAppl : forall v pf ctxt ctxc ctx arg ty curry out,
+      Value v ->
+      PartitionKV pf ctxt ctxc ->
+      ctx = pf ++ ctxc ->
+      match arg with
+      | None => curry = out
+      | Some x => subst x v curry = Some out
+      end ->
+      Step ctx (TmAppl (TmForA arg ty curry) v) ctxc out
+  | StepApplF : forall ctxf f ctxf' f' ctxx ctx ctx' x,
+      Step ctxf f ctxf' f' ->
+      ctxf ++ ctxx = ctx ->
+      ctxf' ++ ctxx = ctx' ->
+      Step ctx (TmAppl f x) ctx' (TmAppl f' x)
+  | StepApplX : forall ctxx x ctxx' x' ctxf ctx ctx' f,
+      Step ctxx x ctxx' x' ->
+      ctxf ++ ctxx = ctx ->
+      ctxf ++ ctxx' = ctx' ->
+      Step ctx (TmAppl f x) ctx' (TmAppl f x')
+  .
+
+(* Reflexive transitive closure on `Step` *)
+Inductive MultiStep : list (string * term) -> term -> list (string * term) -> term -> Prop :=
+  | MultiStepRefl : forall ctx t,
+      MultiStep ctx t ctx t
+  | MultiStepTrans : forall ctx t ctx' t' ctx'' t'',
+      Step ctx t ctx' t' ->
+      MultiStep ctx' t' ctx'' t'' ->
+      MultiStep ctx t ctx'' t''
+  .
+
+Theorem values_cant_step : forall v,
+  Value v ->
+  forall ctx ctx' v',
+  ~Step ctx v ctx' v'.
+Proof.
+  intros v Hv. induction Hv; intros; simpl in *; intro C; try solve [invert C].
+  - invert C. eapply IHHv. apply H7.
+  - invert C; [eapply IHHv1 | eapply IHHv2]; apply H5.
+  - invert C; [eapply IHHv1 | eapply IHHv2]; apply H1.
+Qed.
