theories/StructuralFreeVariables.v
@@ -1,0 +1,214 @@
+From Coq Require Export
+  Lists.List.
+Export ListNotations.
+From Lang Require Import
+  Invert
+  Terms.
+
+Fixpoint remove_all x li :=
+  match li with
+  | [] => []
+  | hd :: tl =>
+      let recursed := remove_all x tl in
+      if eqb x hd then recursed else hd :: recursed
+  end.
+(* tail-recursive version flips the order *)
+
+Theorem in_remove_all : forall x li,
+  ~In x (remove_all x li).
+Proof.
+  intros x li C. generalize dependent x. induction li; intros; simpl in *. { destruct C. }
+  destruct (eqb_spec x a). { apply IHli in C as []. } destruct C. { subst. apply n. reflexivity. } apply IHli in H as [].
+Qed.
+
+Theorem in_remove_all_neq : forall x y li,
+  x <> y ->
+  (In x (remove_all y li) <-> In x li).
+Proof.
+  intros x y li H. generalize dependent x. generalize dependent y. induction li; intros; simpl in *. { split; intros []. }
+  destruct (eqb_spec y a).
+  - subst. split; intros.
+    + right. eapply IHli. { apply H. } assumption.
+    + destruct H0. { subst. contradiction H. reflexivity. } apply IHli; assumption.
+  - split; intros H0; (destruct H0; [left; assumption |]; right; eapply IHli; [apply H | assumption]).
+Qed.
+
+Fixpoint structural_fv t :=
+  match t with
+  | TmVoid
+  | TmStar _
+  | TmAtom _ =>
+      []
+  | TmVarS s =>
+      [s]
+  | TmAppl f x =>
+      structural_fv f ++ structural_fv x
+  | TmPack _ arg ty curry
+  | TmForA arg ty curry =>
+      structural_fv ty ++ (
+        let recursed := structural_fv curry in
+        match arg with
+        | None => recursed
+        | Some a => remove_all a recursed
+        end)
+  end.
+
+(* Crucial distinction from an easier-to-implement algorithm! *)
+Example structural_fv_permits_shadowing : forall x,
+  (* Equivalent to `\x. \x. x x`, where the `x`s are distinct and pushed/popped in order. *)
+  structural_fv (TmForA (Some x) TmVoid (TmForA (Some x) TmVoid (TmAppl (TmVarS x) (TmVarS x)))) = [].
+Proof. intros. simpl. repeat rewrite eqb_refl. reflexivity. Qed.
+
+(* Crucial distinction from an easier-to-implement algorithm! *)
+Example structural_fv_permits_interrupted_shadowing : forall x y, y <> x ->
+  (* Equivalent to `\x. \y. \x. x x`, where the `x`s are distinct and pushed/popped in order. *)
+  structural_fv (TmForA (Some x) TmVoid (TmForA (Some y) TmVoid (TmForA (Some x) TmVoid (TmAppl (TmVarS x) (TmVarS x))))) = [].
+Proof. intros. simpl. rewrite eqb_refl. reflexivity. Qed.
+
+Example structural_fv_respects_scope : forall x,
+  (* Equivalent to `(\x:0. 0) x`, in which the outer `x` is still free *)
+  structural_fv (TmAppl (TmForA (Some x) TmVoid TmVoid) (TmVarS x)) = [x].
+Proof. intros. simpl. reflexivity. Qed.
+
+(*
+Fixpoint structural_fv_fast acc t :=
+  match t with
+  | TmVoid
+  | TmStar _
+  | TmAtom _ =>
+      acc
+  | TmVarS s =>
+      s :: acc
+  | TmPack _ None a b
+  | TmForA None a b
+  | TmAppl a b =>
+      structural_fv_fast (structural_fv_fast acc b) a
+  | TmPack _ (Some arg) ty curry
+  | TmForA (Some arg) ty curry =>
+      structural_fv_fast (remove_if_head arg (structural_fv_fast acc curry)) ty
+  end.
+
+(* Crucial distinction from an easier-to-implement algorithm! *)
+Example structural_fv_fast_permits_shadowing : forall x,
+  (* Equivalent to `\x. \x. x x`, where the `x`s are distinct and pushed/popped in order. *)
+  structural_fv_fast [] (TmForA (Some x) TmVoid (TmForA (Some x) TmVoid (TmAppl (TmVarS x) (TmVarS x)))) = [].
+Proof. intros. simpl. repeat rewrite eqb_refl. reflexivity. Qed.
+
+(* Crucial distinction from an easier-to-implement algorithm! *)
+Example structural_fv_fast_permits_interrupted_shadowing : forall x y, y <> x ->
+  (* Equivalent to `\x. \y. \x. x x`, where the `x`s are distinct and pushed/popped in order. *)
+  structural_fv_fast [] (TmForA (Some x) TmVoid (TmForA (Some y) TmVoid (TmForA (Some x) TmVoid (TmAppl (TmVarS x) (TmVarS x))))) = [].
+Proof. intros. apply eqb_neq in H. simpl. rewrite eqb_refl. rewrite H. rewrite eqb_refl. reflexivity. Qed.
+
+Example structural_fv_fast_respects_scope : forall x,
+  (* Equivalent to `(\x:0. 0) x`, in which the outer `x` is still free *)
+  structural_fv_fast [] (TmAppl (TmForA (Some x) TmVoid TmVoid) (TmVarS x)) = [x].
+Proof. intros. simpl. Abort.
+
+Theorem structural_fv_fast_slow_eq : forall t,
+  structural_fv_slow t = rev (snd (structural_fv_fast [] [] t)).
+Proof.
+  intros t. induction t; intros; simpl in *; try reflexivity.
+  - destruct arg.
+    + destruct (structural_fv_slow t2).
+      * rewrite app_nil_r. rewrite IHt1. destruct (structural_fv_fast [] [] t1).
+Qed.
+
+Definition structural_fv := structural_fv_fast [].
+*)
+
+Inductive Wherever {T} (x : T) : list T -> list T -> Prop :=
+  | WhereverNil :
+      Wherever x [] []
+  | WhereverHere : forall a b,
+      Wherever x a b ->
+      Wherever x a (x :: b)
+  | WhereverSkip : forall hd tla tlb,
+      x <> hd ->
+      Wherever x tla tlb ->
+      Wherever x (hd :: tla) (hd :: tlb)
+  .
+
+Example wherever_12345 : Wherever 9 [1;2;3;4;5] [9;1;9;9;2;3;9;4;9;9;9;9;5;9].
+Proof. repeat constructor; intro C; discriminate C. Qed.
+
+Lemma wherever_refl : forall {T} (x : T) li,
+  (~In x li) ->
+  Wherever x li li.
+Proof.
+  induction li; constructor; apply Decidable.not_or in H as [H I]. { symmetry. assumption. } apply IHli. assumption.
+Qed.
+
+Lemma wherever_not_in_orig : forall {T} (x : T) li post,
+  Wherever x li post ->
+  ~In x li.
+Proof.
+  intros T x li post H C. generalize dependent C. generalize dependent post. generalize dependent x.
+  induction li; intros; destruct C; subst.
+  - remember (x :: li) as xli eqn:Ex. induction H; intros.
+    { discriminate. } { apply IHWherever. assumption. } invert Ex. apply H. reflexivity.
+  - remember (a :: li) as ali eqn:Ea. generalize dependent a. generalize dependent li. induction H; intros.
+    { discriminate. } { eapply IHWherever. { apply IHli. } { assumption. } apply Ea. }
+    invert Ea. eapply IHli. { apply H0. } assumption.
+Qed.
+
+Lemma wherever_remove_all : forall x li post,
+  Wherever x li post <-> remove_all x post = li.
+Proof.
+  split; intros.
+  - induction H.
+    + reflexivity.
+    + simpl. rewrite eqb_refl. assumption.
+    + simpl. apply eqb_neq in H. rewrite H. f_equal. assumption.
+  - generalize dependent x. generalize dependent li. induction post; intros.
+    + invert H. constructor.
+    + simpl in H. destruct (eqb x a) eqn:E.
+      * apply eqb_eq in E. subst. constructor. apply IHpost. reflexivity.
+      * apply eqb_neq in E. subst. constructor. { assumption. } apply IHpost. reflexivity.
+Qed.
+
+Inductive StructurallyFreeIn : term -> list string -> Prop :=
+  | FreeVoid :
+      StructurallyFreeIn TmVoid []
+  | FreeStar : forall univ,
+      StructurallyFreeIn (TmStar univ) []
+  | FreeAtom : forall id,
+      StructurallyFreeIn (TmAtom id) []
+  | FreeVarS : forall x,
+      StructurallyFreeIn (TmVarS x) [x]
+  | FreePack : forall id arg ty curry v,
+      StructurallyFreeIn (TmForA    arg ty curry) v ->
+      StructurallyFreeIn (TmPack id arg ty curry) v
+  | FreeForA : forall arg ty curry va vb avb v,
+      StructurallyFreeIn ty va ->
+      StructurallyFreeIn curry avb ->
+      (match arg with None => eq | Some a => Wherever a end) vb avb ->
+      v = va ++ vb ->
+      StructurallyFreeIn (TmForA arg ty curry) v
+  | FreeAppl : forall f x va vb v,
+      StructurallyFreeIn f va ->
+      StructurallyFreeIn x vb ->
+      va ++ vb = v ->
+      StructurallyFreeIn (TmAppl f x) v
+  .
+Arguments StructurallyFreeIn t vs.
+
+Definition ClosedStructural := fun t => StructurallyFreeIn t [].
+Arguments ClosedStructural t/.
+
+Lemma map_distr : forall {A B} (f : A -> B) hd tl, map f (hd ++ tl) = map f hd ++ map f tl.
+Proof.
+  intros. generalize dependent tl. generalize dependent B.
+  induction hd; intros; simpl in *; try rewrite IHhd; reflexivity.
+Qed.
+
+Theorem reflect_structural_fv : forall t v,
+  structural_fv t = v <-> StructurallyFreeIn t v.
+Proof.
+  split; intros.
+  - generalize dependent v. induction t; intros; subst; simpl in *; try constructor;
+    econstructor; try apply IHt1; try apply IHt2; try reflexivity;
+    (destruct arg; [| reflexivity]); apply wherever_remove_all; reflexivity.
+  - induction H; subst; simpl in *; try reflexivity. destruct arg; [| subst; reflexivity].
+    apply wherever_remove_all in H1. subst. reflexivity.
+Qed.
