theories/StructuralSubst.v
@@ -1,0 +1,242 @@
+From Coq Require Export
+  List.
+Export ListNotations.
+From Lang Require Import
+  FstCmp
+  Invert
+  StructuralFreeVariables
+  Terms.
+
+Fixpoint smap
+  (f : (term -> term) -> term -> term)
+  (x : list (string * (term -> term))) :
+  list (string * (term -> term)) :=
+  match x with
+  | [] => []
+  | (s, g) :: tl => (s, f g) :: smap f tl
+  end.
+
+Theorem smap_distr : forall f a b,
+  smap f (a ++ b) = smap f a ++ smap f b.
+Proof.
+  intros f a. generalize dependent f. induction a; intros; simpl in *.
+  { reflexivity. } destruct a. rewrite IHa. reflexivity.
+Qed.
+
+Theorem smap_len : forall f li,
+  Datatypes.length (smap f li) = Datatypes.length li.
+Proof.
+  intros f li. generalize dependent f. induction li; intros; simpl in *.
+  { reflexivity. } destruct a. simpl. rewrite IHli. reflexivity.
+Qed.
+
+Theorem map_fst_smap : forall f li,
+  map fst (smap f li) = map fst li.
+Proof. induction li. { reflexivity. } destruct a. simpl. rewrite IHli. reflexivity. Qed.
+
+Fixpoint remove_key_all {T} x (li : list (string * T)) :=
+  match li with
+  | [] => []
+  | (s, f) :: tl =>
+      let recursed := remove_key_all x tl in
+      if eqb x s then recursed else (s, f) :: recursed
+  end.
+
+Lemma remove_all_key_eq : forall {T} x (li : list (string * T)),
+  map fst (remove_key_all x li) = remove_all x (map fst li).
+Proof.
+  intros. generalize dependent x. induction li; intros; simpl in *. { reflexivity. }
+  destruct a. simpl. destruct (eqb x s) eqn:E. { apply IHli. } simpl. f_equal. apply IHli.
+Qed.
+
+Lemma remove_key_all_eq : forall {T} x li,
+  ~In x (map fst li) ->
+  @remove_key_all T x li = li.
+Proof.
+  intros. generalize dependent x. induction li; intros; simpl in *. { reflexivity. }
+  destruct a. simpl in *. apply Decidable.not_or in H as [H1 H2]. apply eqb_neq in H1.
+  rewrite eqb_sym in H1. rewrite H1. f_equal. apply IHli. assumption.
+Qed.
+
+(* Ludicrous that this is the easiest correct definition to write.
+ * Generates substitution functions for every free variable at once. *)
+Fixpoint structural_grand_unified_subst t : list (string * (term -> term)) :=
+  match t with
+  | TmVoid
+  | TmStar _
+  | TmAtom _ =>
+      []
+  | TmVarS s =>
+      [(s, fun x => x)]
+  | TmPack id arg ty curry =>
+      smap (fun f x => TmPack id arg (f x) curry) (structural_grand_unified_subst ty) ++
+      smap (fun f x => TmPack id arg ty (f x)) (
+        let recursed := structural_grand_unified_subst curry in
+        match arg with
+        | None => recursed
+        | Some a => remove_key_all a recursed
+        end)
+  | TmForA arg ty body =>
+      smap (fun f x => TmForA arg (f x) body) (structural_grand_unified_subst ty) ++
+      smap (fun f x => TmForA arg ty (f x)) (
+        let recursed := structural_grand_unified_subst body in
+        match arg with
+        | None => recursed
+        | Some a => remove_key_all a recursed
+        end)
+  | TmAppl a b =>
+      smap (fun f x => TmAppl (f x) b) (structural_grand_unified_subst a) ++
+      smap (fun f x => TmAppl a (f x)) (structural_grand_unified_subst b)
+  end.
+
+Fixpoint pair_lookup {V} key (pairs : list (string * V)) :=
+  match pairs with
+  | [] => None
+  | (k, v) :: tl => if eqb key k then Some v else pair_lookup key tl
+  end.
+
+Definition structural_subst x y t := option_map (fun f => f y) (pair_lookup x (structural_grand_unified_subst t)).
+Arguments structural_subst x y t/.
+
+Example structural_subst_simple : forall f x,
+  structural_subst f TmVoid (TmAppl (TmVarS f) x) = Some (TmAppl TmVoid x).
+Proof. intros. simpl. rewrite eqb_refl. reflexivity. Qed.
+
+Example structural_grand_unified_subst_simple :
+  structural_grand_unified_subst (TmAppl (TmVarS "f"%string) (TmVarS "x"%string)) = [
+    ("f"%string, fun t => TmAppl t (TmVarS "x"%string));
+    ("x"%string, fun t => TmAppl (TmVarS "f"%string) t)].
+Proof. reflexivity. Qed.
+
+Example structural_grand_unified_subst_lambda :
+  structural_grand_unified_subst (TmForA (Some "x") (TmVarS "T") (TmAppl (TmVarS "x") (TmVarS "x")))%string = [
+    ("T", fun x => TmForA (Some "x") x (TmAppl (TmVarS "x") (TmVarS "x")))]%string.
+    (* do NOT ignore the first `x`, unlike the non-structural version, even thoguh it's bound *)
+Proof. reflexivity. Qed.
+
+Lemma fst_cmp_eqb : forall {T} a a' b b',
+  @fst_cmp T T (a, b) (a', b') = eqb a a'.
+Proof. reflexivity. Qed.
+
+Theorem structural_grand_unified_subst_fv : forall t,
+  structural_fv t = map fst (structural_grand_unified_subst t).
+Proof.
+  induction t; intros; subst; simpl in *; try reflexivity; repeat rewrite slow_down;
+  repeat rewrite IHt1; repeat rewrite IHt2; repeat rewrite map_distr; repeat rewrite map_fst_smap; [| | reflexivity];
+  destruct arg; f_equal; repeat rewrite <- partition_pf_fast_slow; try rewrite (map_fst_partition_pf _ _ _ _ fst_cmp_eqb);
+  repeat rewrite map_fst_smap; repeat rewrite remove_all_key_eq; reflexivity.
+Qed.
+
+Lemma pair_lookup_smap : forall f x li,
+  pair_lookup x (smap f li) = option_map f (pair_lookup x li).
+Proof.
+  intros f x li. generalize dependent x. generalize dependent f.
+  induction li; intros; simpl in *. { reflexivity. }
+  destruct a. simpl. destruct (eqb x s) eqn:E. { reflexivity. } apply IHli.
+Qed.
+
+Lemma pair_lookup_app : forall {T} x a b,
+  @pair_lookup T x (a ++ b) =
+  match pair_lookup x a with
+  | None => pair_lookup x b
+  | Some out => Some out
+  end.
+Proof.
+  intros T x a. generalize dependent x. induction a; intros; simpl in *. { reflexivity. }
+  destruct a. destruct (eqb x s). { reflexivity. } apply IHa.
+Qed.
+
+Lemma pair_lookup_Forall_snd : forall {T} P li x y,
+  Forall P (map snd li) ->
+  @pair_lookup T x li = Some y ->
+  P y.
+Proof.
+  intros T P li x y Hf Hl. generalize dependent y. generalize dependent x.
+  remember (map snd li) eqn:Emap. generalize dependent li.
+  induction Hf; intros; destruct li; invert Emap; try discriminate Hl.
+  destruct p. simpl in *. destruct (eqb x0 s) eqn:E. { invert Hl. assumption. }
+  eapply IHHf; [reflexivity |]. apply Hl.
+Qed.
+
+Lemma pair_lookup_Forall : forall {T} P li x t,
+  Forall P li ->
+  @pair_lookup T x li = Some t ->
+  P (x, t).
+Proof.
+  intros T P li x t Hf Hl. generalize dependent t. generalize dependent x.
+  induction Hf; intros; simpl in *. { discriminate Hl. } destruct x as [k v].
+  destruct (eqb x0 k) eqn:E; [apply eqb_eq in E; invert Hl | apply IHHf]; assumption.
+Qed.
+
+Theorem Forall_smap : forall f P li,
+  Forall (fun p : _ * _ => let (x, g) := p in P (x, f g)) li ->
+  Forall P (smap f li).
+Proof.
+  intros. remember (fun p : string * (term -> term) => let (x, g) := p in P (x, f g)) as F eqn:EF.
+  generalize dependent P. generalize dependent f. induction H; intros; [apply Forall_nil |].
+  destruct x as [s g]. subst. simpl in *. constructor; [assumption |]. apply IHForall. reflexivity.
+Qed.
+
+Lemma remove_key_all_incl : forall {T} x (li : list (string * T)),
+  incl (remove_key_all x li) li.
+Proof.
+  unfold incl. intros T x li. generalize dependent x. induction li; intros; simpl in *. { destruct H. }
+  destruct a. destruct (eqb x s) eqn:E. { apply eqb_eq in E. subst. right. eapply IHli. apply H. }
+  destruct a0. destruct H. { left. assumption. } right. eapply IHli. apply H.
+Qed.
+
+(* God this is the dumbest function of all time but it's only ever used in proofs *)
+Fixpoint slow_unique_key {T} (li : list (string * T)) :=
+  match li with
+  | [] => []
+  | (s, t) :: tl => (s, t) :: remove_key_all s (slow_unique_key tl)
+  end.
+
+Lemma has_remove_key_all : forall {T} (x y : string * T) (li : list (string * T)),
+  fst_cmp x y = false ->
+  existsb (fst_cmp x) (remove_key_all (fst y) li) = existsb (fst_cmp x) li.
+Proof.
+  intros. generalize dependent y. generalize dependent x. induction li; intros; simpl in *. { reflexivity. }
+  destruct a. destruct x. destruct y. unfold fst_cmp in *. simpl in *.
+  destruct (eqb s1 s) eqn:E1. { apply eqb_eq in E1. subst. rewrite H. apply (IHli (s0, t0) (s, t)). assumption. }
+  destruct (eqb s0 s) eqn:E0; simpl in *. { rewrite E0. reflexivity. } rewrite E0. apply (IHli (s0, t0) (s1, t1)). assumption.
+Qed.
+
+Lemma has_slow_unique : forall {T} x li,
+  existsb (@fst_cmp T T x) (slow_unique_key li) = existsb (fst_cmp x) li.
+Proof.
+  intros T [s t] li. generalize dependent t. generalize dependent s.
+  induction li; intros; simpl in *. { reflexivity. }
+  destruct a. destruct (eqb_spec s s0). { subst. unfold fst_cmp. simpl. rewrite eqb_refl. reflexivity. }
+  simpl. rewrite (has_remove_key_all (s, t) (s0, t0)). 2: { unfold fst_cmp. simpl. apply eqb_neq. assumption. }
+  unfold fst_cmp. simpl. apply eqb_neq in n. rewrite n. apply (IHli _ t).
+Qed.
+
+(*
+Theorem incl_partition_pf_fst : forall {T} hi lo,
+  incl (@partition_pf_slow (string * T) fst_cmp hi lo) hi.
+Proof.
+  unfold incl. induction hi; intros; simpl in *. { destruct H. }
+  destruct (existsb (fst_cmp a) lo) eqn:El; simpl in *. { right. apply (IHhi _ _ H). }
+  destruct (existsb (fst_cmp a) hi) eqn:Eh; simpl in *. { right. apply (IHhi _ _ H). }
+  destruct a as [k1 v1]. destruct a0 as [k2 v2]. destruct H; [| right; apply (IHhi _ _ H)].
+  left. assumption.
+Qed.
+*)
+
+Theorem structural_grand_unified_subst_id : forall t,
+  let P := fun p : _ * _ => let (x, f) := p in f (TmVarS x) = t in
+  Forall P (structural_grand_unified_subst t).
+Proof.
+  induction t as [| | | | id arg a IHa b IHb | arg a IHa b IHb | a IHa b IHb]; simpl in *; repeat constructor;
+  apply Forall_app; split; apply Forall_smap; try (destruct arg; [eapply incl_Forall; [apply remove_key_all_incl |] |]);
+  (eapply Forall_impl; [| try apply IHa; apply IHb]); intros; destruct a0; rewrite H; reflexivity.
+Qed.
+
+Theorem structural_subst_id : forall x t s,
+  structural_subst x (TmVarS x) t = Some s ->
+  s = t.
+Proof.
+  intros. unfold structural_subst in *. destruct (pair_lookup x (structural_grand_unified_subst t)) eqn:Ep; invert H.
+  eapply pair_lookup_Forall in Ep; [| apply structural_grand_unified_subst_id]. assumption.
+Qed.
