theories/StructuralTypes.v
@@ -1,0 +1,187 @@
+From Coq Require Export
+  Lists.List
+  Sorting.Permutation.
+Export ListNotations.
+From Lang Require Import
+  Find
+  StructuralFreeVariables
+  InTactics
+  Invert
+  StructuralSubst
+  Terms.
+
+Variant MaybeStructurallySubst : option string -> term -> term -> term -> Prop :=
+  | MaybeSubstNone : forall y t,
+      MaybeSubst None y t t
+  | MaybeSubstSome : forall t x y t',
+      structural_subst x y t = Some t' ->
+      MaybeSubst (Some x) y t t'
+  .
+
+(* Prevent having two variables with the same name (fst) but different types (snd). *)
+Inductive MaybeConsKV {K V} k v : list (K * V) -> list (K * V) -> Prop :=
+  | MaybeConsKVCons : forall tl,
+      MaybeConsKV k v tl ((k, v) :: tl)
+  | MaybeConsKVNil :
+      MaybeConsKV k v [] []
+  | MaybeConsKVNotEq : forall hdk hdv tl,
+      k <> hdk ->
+      (* `hdv` can be the same, that's fine: two variables can have the same type *)
+      MaybeConsKV k v ((hdk, hdv) :: tl) ((hdk, hdv) :: tl)
+  .
+
+Inductive WhereverKV {K V} k v : list (K * V) -> list (K * V) -> Prop :=
+  | WhereverKeyHere : forall a b,
+      WhereverKV k v a b ->
+      WhereverKV k v a ((k, v) :: b)
+  | WhereverKeyNil :
+      WhereverKV k v [] []
+  | WhereverKeyNotEq : forall hdk hdv a b,
+      k <> hdk ->
+      (* `v` can be the same, that's fine: two variables can have the same type *)
+      WhereverKV k v a b ->
+      WhereverKV k v ((hdk, hdv) :: a) ((hdk, hdv) :: b)
+  .
+
+(* Typed just like in any other programming language (other than Rust). *)
+Inductive StructurallyTyped : list (string * term) -> term -> term -> Prop :=
+  | STyStar : forall ctx univ,
+      StructurallyTyped ctx (TmStar univ) (TmStar (S univ))
+  | STyVarS : forall ctx id t,
+      FindKV id t ctx ->
+      StructurallyTyped ctx (TmVarS id) t
+  | STyAtom : forall ctx id,
+      StructurallyTyped ctx (TmAtom id) (TmAtom id)
+  | STyPack : forall ctx id arg arg_ty curry ty,
+      AtomId id curry ->
+      StructurallyTyped ctx (TmForA    arg arg_ty curry) ty ->
+      StructurallyTyped ctx (TmPack id arg arg_ty curry) ty
+  | STyForA : forall ctx arg ty body t kind,
+      StructurallyTyped ctx ty kind ->
+      StructurallyTyped (match arg with None => ctx | Some a => (a, ty) :: ctx end) body t ->
+      StructurallyTyped ctx (TmForA arg ty body) (TmForA arg ty t)
+  | STyAppl : forall ctx f x arg ty body substituted,
+      StructurallyTyped ctx f (TmForA arg ty body) ->
+      StructurallyTyped ctx x ty ->
+      MaybeSubst arg x body substituted ->
+      StructurallyTyped ctx (TmAppl f x) substituted
+  (*
+  | STyStar : forall ctx t ty,
+      StructurallyTyped ctx t ty ->
+      StructurallyTyped ctx t TmStar
+  *)
+  .
+Arguments StructurallyTyped ctx t ty.
+
+(* TODO: CRUCIAL SAFETY THEOREMS: (1) Star n does not have type Star n, and (2) no term has type Void. *)
+
+(* Polymorphic identity function.
+ * `\t: *. \x: t. x` is typable (!), and in fact it has type
+ * `\t: *. \x: t. t`, almost but not quite the same. Could be simplified to
+ * `\t: *. (t -> t)` by making the `x` anonymous. *)
+Definition polymorphic_identity_fn := (TmForA (Some "t") (TmStar 0) (TmForA (Some "x") (TmVarS "t") (TmVarS "x")))%string.
+Definition polymorphic_identity_ty := (TmForA (Some "t") (TmStar 0) (TmForA (Some "x") (TmVarS "t") (TmVarS "t")))%string.
+Arguments polymorphic_identity_fn/.
+Arguments polymorphic_identity_ty/.
+Theorem dependent_types_woohoo :
+  StructurallyTyped [] polymorphic_identity_fn polymorphic_identity_ty.
+Proof.
+  simpl. eapply STyForA.
+  - (* typing `TmStar` *)
+    apply STyStar.
+  - (* typing the body *)
+    eapply STyForA.
+    + (* typing `TmVarS "t"` *)
+      apply STyVarS. find_kv.
+    + (* typing `TmVarS "x" : TmVarS "t"` *)
+      apply STyVarS. find_kv.
+Qed.
+
+(* Showing that, given f: X -> Y and x: X, we can type (f x) : Y. *)
+Example type_fn_app :
+  let f := TmVarS "f"%string in
+  let x := TmVarS "x"%string in
+  let X := TmVarS "X"%string in
+  let Y := TmVarS "Y"%string in
+  let tf := ("f"%string, TmForA None X Y) in
+  let tx := ("x"%string, X) in
+  let ctx := [tf; tx] in
+  let fx := TmAppl f x in
+  StructurallyTyped ctx fx Y.
+Proof. repeat econstructor. intro C. discriminate C. Qed.
+
+(* ...But the above becomes perfectly okay if we add exchange and contraction, i.e., a heap: *)
+Example structural_type_allows_reuse :
+  let f := TmVarS "f"%string in
+  let x := TmVarS "x"%string in
+  let X := TmVarS "X"%string in
+  let Y := TmVarS "Y"%string in
+  let tf := ("f"%string, TmForA None X (TmForA None X Y)) in
+  let tx := ("x"%string, X) in
+  let ctx := [tf; tx] in
+  let fxx := TmAppl (TmAppl f x) x in
+  StructurallyTyped ctx fxx Y.
+Proof.
+  simpl. eapply STyAppl.
+  - eapply STyAppl.
+    + apply STyVarS. find_kv.
+    + apply STyVarS. find_kv.
+    + apply MaybeSubstNone.
+  - apply STyVarS. find_kv.
+  - apply MaybeSubstNone.
+Qed.
+
+Lemma wherever_fst : forall {A B} f s li post,
+  @WhereverKV A B s f            li           post ->
+  @Wherever   A   s     (map fst li) (map fst post).
+Proof. intros. induction H; constructor; assumption. Qed.
+
+Theorem structurally_typed_fv : forall ctx t ty,
+  StructurallyTyped ctx t ty ->
+  incl (fv_with remove_all t) (map fst ctx).
+Proof.
+  unfold incl. intros. generalize dependent a. induction H; intros; simpl in *; repeat rewrite slow_down in *;
+  try solve [destruct H0]; try (destruct H0; [| destruct H0]; subst; eapply find_kv_in_fst; apply H).
+  { apply IHStructurallyTyped. assumption. } 2: {
+    apply in_app_iff in H2. destruct H2; [apply IHStructurallyTyped1 | apply IHStructurallyTyped2]; assumption. }
+  destruct arg; simpl in *. 2: {
+    induction (fv_with remove_all ty); simpl in *. { apply IHStructurallyTyped2. assumption. }
+    destruct (existsb (eqb a0) (fv_with remove_all body) || existsb (eqb a0) l)%bool eqn:E; [| destruct H1];
+    try (apply IHl; [| assumption]; intros; apply IHStructurallyTyped1; right; assumption).
+    apply IHStructurallyTyped1. left. assumption. }
+  induction (fv_with remove_all ty); simpl in *.
+  - destruct (eqb_spec s a). { subst. apply in_remove_all in H1 as []. }
+    apply in_remove_all_neq in H1; [| intro C; subst; contradiction n; reflexivity].
+    apply IHStructurallyTyped2 in H1. destruct H1. { subst. contradiction n. reflexivity. } assumption.
+  - destruct (existsb_in eqb a0 (remove_all s (fv_with remove_all body)) eqb_spec);
+    destruct (existsb_in eqb a0 l eqb_spec); [| | | destruct H1];
+    try (apply IHl; [| assumption]; intros; apply IHStructurallyTyped1; right; assumption).
+    apply IHStructurallyTyped1. left. assumption.
+Qed.
+
+Theorem fv_not_typed : forall ctx t,
+  (~incl (fv_with remove_all t) (map fst ctx)) -> ~exists ty, StructurallyTyped ctx t ty.
+Proof.
+  unfold incl. intros ctx t H [ty C]. generalize dependent H. induction C; intros; simpl in *; try rewrite slow_down in *.
+  - apply H. intros. destruct H0.
+  - induction H.
+    + apply H0. intros. destruct H; [| destruct H]. subst. left. reflexivity.
+    + apply IHFindKV. intro C. apply H0. intros. destruct H2; [| destruct H2]. subst. right. apply C. left. reflexivity.
+  - apply H. intros. destruct H0.
+  - apply IHC. assumption.
+  - admit.
+  - apply H0. intros. apply in_app_iff in H1. destruct H1.
+    + contradiction IHC1. intro C. apply H0. intros. apply C. apply C in H1.
+
+  intros t H [ty C]. remember (@nil (string * term)) as ctx eqn:Ec. generalize dependent Ec. generalize dependent H.
+  induction C; intros; subst; simpl in *; try (apply H; reflexivity); try solve [inversion H]; try rewrite slow_down in *.
+  { apply IHC; [| reflexivity]. assumption. } 2: {
+    destruct (fv_with remove_all f). { apply IHC2; [| reflexivity]. assumption. }
+    apply IHC1; [| reflexivity]. intro C. discriminate C. }
+  destruct arg; simpl in *. 2: {
+    destruct (fv_with remove_all ty); [| apply IHC1; [| reflexivity]; intro C; discriminate C].
+    destruct (fv_with remove_all body). { apply H. reflexivity. } apply IHC2; [| reflexivity]. intro C. discriminate C. }
+  clear IHC2. destruct (fv_with remove_all ty); simpl in *. 2:{ apply IHC1; [| reflexivity]. intro C. discriminate C. }
+  clear IHC1. Abort. (* TODO *)
+
+(* TODO: Substitution (WITH STRUCTURAL RULES, NOT JUST THE USUAL FUNCTION) preserves typing *)
