theories/TypeSafety.v
@@ -1,7 +1,56 @@
 From Lang Require Import
+  Find
   Invert
+  PartitionKV
+  Step
   Terms
-  Types.
+  Types
+  Values.
+
+Lemma typed_empty_wherever : forall t ty,
+  Typed [] t ty ->
+  TypedWith WhereverKV [] [] t ty.
+Proof.
+  intros. simpl in *. remember MaybeConsKV as m eqn:Em. generalize dependent Em.
+  remember [] as e eqn:Ee. generalize dependent Ee.
+  remember [] as c eqn:Ec. generalize dependent Ec.
+  induction H; intros; subst; simpl in *; try solve [constructor]; try contradiction H.
+  1:{ constructor. { assumption. } apply IHTypedWith; reflexivity. }
+  2:{ destruct ctxf; destruct ctxx; invert Ec.
+      econstructor; [apply IHTypedWith1 | apply IHTypedWith2 | | assumption]; reflexivity. }
+  destruct pf; destruct ctxc; invert Ec. invert H2; [| invert H3 | invert H4].
+  econstructor; [apply H | | destruct arg; [constructor | reflexivity] | apply PartitionKVDone | reflexivity].
+  destruct arg. 2: { subst. apply IHTypedWith2; reflexivity. } invert H1. 2: { apply IHTypedWith2; reflexivity. }
+Abort.
+
+Theorem values_always_typed : forall v,
+  Value v ->
+  exists ty, Typed [] v ty.
+Proof.
+  intros. induction H.
+  1:{ exists (TmStar (S univ)). constructor. }
+  1:{ exists (TmAtom id). constructor. }
+  1:{ destruct IHValue as [t IH]. exists t. econstructor; assumption. }
+  2:{ destruct IHValue1 as [t1 H1]. destruct IHValue2 as [t2 H2]. invert H1; [| destruct H3]. invert H10; [| destruct H1].
+      destruct pf; destruct ctxc; invert H13. invert H12; [| invert H1 | invert H3]. eexists. econstructor.
+      1:{ constructor. { assumption. } econstructor. { apply H5. } { apply H6. } { apply H8. } { constructor. } reflexivity. }
+      2:{ reflexivity. }
+      econstructor. { constructor. { assumption. } invert H10. apply H10.
+  - destruct IHValue1 as [t1 IH1]. destruct IHValue2 as [t2 IH2]. eexists.
+    econstructor; [| apply IH2 | destruct arg; [apply MaybeConsKVNil | reflexivity] | apply PartitionKVDone | reflexivity].
+  - exists ty. assumption.
+Qed.
+
+Theorem progress : forall ctx t ty,
+  Typed ctx t ty ->
+  (Value t \/ exists ctx' t', Step ctx t ctx' t').
+Proof.
+  intros ctx t ty Ht. induction Ht; intros; simpl in *.
+  - left. constructor.
+  - right. exists []. exists t. constructor.
+  - left. constructor.
+  - right. left. constructor.
+Qed.
 
 (*
 Theorem no_type_in_type : forall ctx,
